<?xml version="1.0"?>
<section xml:id="chapter5_one-more-example">
  <title>One more example</title>
  <p>In the previous example I used temporary variables to spell out the
            steps, and to make the code easier to debug, but I could have saved a
            few lines:</p>
  <exercise label="recursion_ex_AC_1">
    <statement>
      <p>This program uses recursion to calculate the factorial of
            the passed argument.  It is the condensed version of the
            example on the previous page.</p>
    </statement>
    <program xml:id="recursion_ex_AC_1_editor" interactive="activecode" language="cpp" line-numbers="yes">
      <input><![CDATA[
#include <iostream>
using namespace std;

int factorial (int n) {
    if (n == 0) {
        return 1;
    }
    else {
        return n * factorial (n-1);
    }
}

int main () {
    cout << factorial(3) << endl;
}
        ]]></input>
    </program>
  </exercise>
  <p>From now on I will tend to use the more concise version, but I recommend
            that you use the more explicit version while you are developing code.
            When you have it working, you can tighten it up, if you are feeling
            inspired.</p>
  <p>After factorial, the classic example of a recursively-defined
            mathematical function is fibonacci, which has the following definition:</p>
  <math_block docname="Chapter5/onemoreexample" label="True" nowrap="False" number="True" xml:space="preserve">\begin{aligned}
&amp;&amp; fibonacci(0) = 1 \\
&amp;&amp; fibonacci(1) = 1 \\
&amp;&amp; fibonacci(n) = fibonacci(n-1) + fibonacci(n-2);\end{aligned}</math_block>
  <p>Translated into C++, this is</p>
  <exercise label="recursion_ex_AC_2">
    <statement>
      <p>This program uses recursion to calculate the nth number in the
            fibonacci sequence.</p>
    </statement>
    <program xml:id="recursion_ex_AC_2_editor" interactive="activecode" language="cpp" line-numbers="yes">
      <input><![CDATA[
#include <iostream>
using namespace std;

int fibonacci (int n) {
    if (n == 0 || n == 1) {
        return 1;
    }
    else {
        return fibonacci (n-1) + fibonacci (n-2);
    }
}

int main () {
    cout << fibonacci(3) << endl;
}
        ]]></input>
    </program>
  </exercise>
  <p>If you try to follow the flow of execution here, even for fairly small
            values of n, your head explodes. But according to the leap of faith, if
            we assume that the two recursive calls (yes, you can make two recursive
            calls) work correctly, then it is clear that we get the right result by
            adding them together.</p>
</section>
